theories/Reflection2/PredMonadState.v
@@ -28,8 +28,30 @@ Class PredMonadState M PM St {OM: OTypeF1 M} {OPM: OTypeF1 PM} {OSt: OType St}
  *** Hoare Logic using Predicate Monads
  ***)
 
+(* FIXME HERE NOW: move to Monad.v *)
+Notation "'edo' x <- m1 ; m2" :=
+  (Embed bindM @e@ m1 @e@ (mkLam (fun x => m2)))
+    (at level 60, right associativity).
+
+Definition evalExpr {A RA} (e:@OExpr CtxNil A RA) : A :=
+  exprSemantics e @o@ tt.
+Arguments evalExpr {A RA} !e.
+
 Definition HoareP `{PredMonadState} `{OType} :
   (St -o> Flip Prop) -o> (St -o> A -o> St -o> Prop) -o> PM A _ :=
+  evalExpr
+    (efun pre =>
+     efun post =>
+     edo s_pre <- Embed getM ;
+       (Embed assumingP)
+         @e@ (pre _ _ @e@ s_pre _ _)
+         @e@ (edo x <- Embed trueP;
+                edo s_post <- Embed getM;
+                edo unused
+                    <- Embed assertP @e@ (post _ _ @e@ s_pre _ _
+                                               @e@ x _ _ @e@ s_post _ _);
+                Embed returnM @e@ x _ _)).
+  (*
   ofun pre =>
   ofun post =>
   do s_pre <- getM;
@@ -40,3 +62,4 @@ Definition HoareP `{PredMonadState} `{OType} :
              do unused
                 <- assertP @o@ (post @o@ s_pre @o@ x @o@ s_post);
              returnM @o@ x).
+   *)
